Add a BBM success test case (with DSB, ISB, TLBI) - Update sail-tiny-arm commit hash - Refactor tests

ArchSemArm/tests/VMPromisingTest.v
@@ -90,6 +90,33 @@ Definition table_desc (next_pa : Z) : Z :=
 Definition page_desc (out_pa : Z) : Z :=
   Z.lor (Z.lor (Z.land out_pa (Z.lnot 0xFFF%Z)) 0x400%Z) 0x3%Z.  (* Valid=1, Page=1, AF=1 *)
 
+Definition init_empty_table (mem : memoryMap) (baddr : bv addr_size) : memoryMap :=
+  let reserved_addrs := dom mem in
+  foldl (λ mem index,
+    let addr := baddr `+Z` (index * 8) in
+    if decide (addr ∈ reserved_addrs)
+    then mem
+    else mem_insert addr 8 0 mem) mem (seqZ 0 512).
+
+Definition clear_offset (addr : bv addr_size) : bv addr_size :=
+  let ones : bv 9 := (-1)%bv in
+  bv_and addr (bv_not (bv_zero_extend addr_size ones)).
+
+Definition init_vmem (instrs : list (bv addr_size * bv 32))
+      (data : list (bv addr_size * bv 64))
+      (pgt : list (bv addr_size * bv 64))
+      (mem_strict : bool) : memoryMap :=
+  let mem_instrs :=
+    foldl (λ mem '(addr, val), mem_insert addr 4 val mem) ∅ instrs in
+  let mem :=
+    foldl (λ mem '(addr, val), mem_insert addr 8 val mem) mem_instrs (data ++ pgt) in
+
+  (* WARNING: initialising 512 entries make tests slow *)
+  if mem_strict then
+    let baddrs := remove_dups $ map clear_offset pgt.*1 in
+    foldl init_empty_table mem baddrs
+  else mem.
+
 (** We test against the sail-tiny-arm semantic, with non-determinism enabled *)
 Definition arm_sem := sail_tiny_arm_sem true.
 
@@ -154,17 +181,16 @@ Module EOR.
     |> reg_insert ID_AA64MMFR1_EL1 0x0
     |> reg_insert PSTATE (init_pstate 0%bv 0%bv).
 
-  Definition init_mem : memoryMap :=
-    ∅
-    |> mem_insert 0x500 4 0xca020020 (* EOR X0, X1, X2 *)
-    (* L0[1] -> L1  (for VA_PC path: L0 index = 1) *)
-    |> mem_insert 0x80008 8 0x81803
-    (* L1[0] -> L2 *)
-    |> mem_insert 0x81000 8 0x82803
-    (* L2[0] -> L3 *)
-    |> mem_insert 0x82000 8 0x83803
-    (* L3[0] : map VA_PC page -> PA page 0x0000 (executable) *)
-    |> mem_insert 0x83000 8 0x403.
+  (* Instruction *)
+  Definition instrs : list (bv addr_size * bv 32) :=
+    [(0x500, 0xca020020) (* EOR X0, X1, X2 *)].
+
+  (* Page table: VA 0x8000000500 to PA 0x500 *)
+  Definition pgt : list (bv addr_size * bv 64) :=
+    [(0x80008, 0x81803); (* L0[1] -> L1 *)
+     (0x81000, 0x82803); (* L1[0] -> L2 *)
+     (0x82000, 0x83803); (* L2[0] -> L3 *)
+     (0x83000, 0x403)]. (* L3[0] -> PA 0x0000 (code page for PC) *)
 
   Definition n_threads := 1%nat.
 
@@ -176,7 +202,7 @@ Module EOR.
   Definition mem_strict := false.
 
   Definition initState :=
-    {|archState.memory := init_mem;
+    {|archState.memory := init_vmem instrs [] pgt mem_strict;
       archState.regs := [# init_reg];
       archState.address_space := PAS_NonSecure |}.
 
@@ -214,20 +240,20 @@ Module LDR.
     |> reg_insert ID_AA64MMFR1_EL1 0x0
     |> reg_insert PSTATE (init_pstate 0%bv 0%bv).
 
-  Definition init_mem : memoryMap:=
-    ∅
-    |> mem_insert 0x500 4 0xf8606820 (* LDR X0, [X1, X0] *)
-    |> mem_insert 0x1000 8 0x2a (* data to be read *)
-    (* L0[1] -> L1  (for VA with L0 index = 1) *)
-    |> mem_insert 0x80008 8 0x81803
-    (* L1[0] -> L2 *)
-    |> mem_insert 0x81000 8 0x82803
-    (* L2[0] -> L3 *)
-    |> mem_insert 0x82000 8 0x83803
-    (* L3[0] : map VA page 0x8000000000 -> PA page 0x0000 (executable, readable) *)
-    |> mem_insert 0x83000 8 0x403
-    (* L3[1] : map VA page 0x8000001000 -> PA page 0x1000 (data, readable, non-executable) *)
-    |> mem_insert 0x83008 8 0x60000000001443.
+  Definition instrs : list (bv addr_size * bv 32) :=
+    [(0x500, 0xf8606820) (* LDR X0, [X1, X0] *)].
+
+  (* Data to be read *)
+  Definition data : list (bv addr_size * bv 64) := [(0x1000, 0x2a)].
+
+  (* Page Table *)
+  Definition pgt : list (bv addr_size * bv 64) :=
+    [(0x80008, 0x81803);
+     (0x81000, 0x82803);
+     (0x82000, 0x83803);
+     (0x83000, 0x403); (* PA page 0x0000 (executable, readable) *)
+     (0x83008, 0x60000000001443) (* PA page 0x1000 (data, readable, non-executable) *)
+    ].
 
   Definition n_threads := 1%nat.
 
@@ -239,7 +265,7 @@ Module LDR.
   Definition mem_strict := false.
 
   Definition initState :=
-    {|archState.memory := init_mem;
+    {|archState.memory := init_vmem instrs data pgt mem_strict;
       archState.regs := [# init_reg];
       archState.address_space := PAS_NonSecure |}.
 
@@ -275,21 +301,22 @@ Module STRLDR.
     |> reg_insert ID_AA64MMFR1_EL1 0x0
     |> reg_insert PSTATE (init_pstate 0%bv 0%bv).
 
-  Definition init_mem : memoryMap:=
-    ∅
-    |> mem_insert 0x500 4 0xf8206822 (* STR X2, [X1, X0] *)
-    |> mem_insert 0x504 4 0xf8606820 (* LDR X0, [X1, X0] *)
-    |> mem_insert 0x1100 8 0x0 (* Memory need to exists to be written to *)
-    (* L0[1] -> L1  (for VA with L0 index = 1) *)
-    |> mem_insert 0x80008 8 0x81803
-    (* L1[0] -> L2 *)
-    |> mem_insert 0x81000 8 0x82803
-    (* L2[0] -> L3 *)
-    |> mem_insert 0x82000 8 0x83803
-    (* L3[0] : map VA page 0x8000000000 -> PA page 0x0000 (executable, readable) *)
-    |> mem_insert 0x83000 8 0x403
-    (* L3[1] : map VA page 0x8000001000 -> PA page 0x1000 (data, readable, non-executable) *)
-    |> mem_insert 0x83008 8 0x60000000001443.
+  (* Instructions *)
+  Definition instrs : list (bv addr_size * bv 32) :=
+    [(0x500, 0xf8206822); (* STR X2, [X1, X0] *)
+     (0x504, 0xf8606820)]. (* LDR X0, [X1, X0] *)
+
+  (* Data to be read *)
+  Definition data : list (bv addr_size * bv 64) := [(0x1100, 0x0)].
+
+  (* Page Table *)
+  Definition pgt : list (bv addr_size * bv 64) :=
+    [(0x80008, 0x81803);
+     (0x81000, 0x82803);
+     (0x82000, 0x83803);
+     (0x83000, 0x403); (* PA page 0x0000 (executable, readable) *)
+     (0x83008, 0x60000000001443) (* PA page 0x1000 (data, readable, non-executable) *)
+    ].
 
   Definition n_threads := 1%nat.
 
@@ -301,7 +328,7 @@ Module STRLDR.
   Definition mem_strict := false.
 
   Definition initState :=
-    {|archState.memory := init_mem;
+    {|archState.memory := init_vmem instrs data pgt mem_strict;
       archState.regs := [# init_reg];
       archState.address_space := PAS_NonSecure |}.
 
@@ -326,10 +353,6 @@ Module MP.
   (* A classic MP litmus test with address translation
      Thread 1: STR X2, [X1, X0]; STR X5, [X4, X3]
      Thread 2: LDR X5, [X4, X3]; LDR X2, [X1, X0]
-
-     VAs map to PAs:
-     - Instructions: 0x8000000500 -> 0x500, 0x8000000600 -> 0x600
-     - Data: 0x8000001100 -> 0x1100, 0x8000001200 -> 0x1200
 
      Expected outcome of (R5, R2) at Thread 2:
       (0x1, 0x2a), (0x0, 0x2a), (0x0, 0x0), (0x1, 0x0)
@@ -365,27 +388,26 @@ Module MP.
     |> reg_insert ID_AA64MMFR1_EL1 0x0
     |> reg_insert PSTATE (init_pstate 0%bv 0%bv).
 
-  Definition init_mem : memoryMap :=
-    ∅
-    (* Thread 1 @ PA 0x500 *)
-    |> mem_insert 0x500 4 0xf8206822  (* STR X2, [X1, X0] *)
-    |> mem_insert 0x504 4 0xf8236885  (* STR X5, [X4, X3] *)
-    (* Thread 2 @ PA 0x600 *)
-    |> mem_insert 0x600 4 0xf8636885  (* LDR X5, [X4, X3] *)
-    |> mem_insert 0x604 4 0xf8606822  (* LDR X2, [X1, X0] *)
-    (* Backing memory so the addresses exist *)
-    |> mem_insert 0x1100 8 0x0
-    |> mem_insert 0x1200 8 0x0
-    (* L0[1] -> L1  (for VA with L0 index = 1) *)
-    |> mem_insert 0x80008 8 0x81803
-    (* L1[0] -> L2 *)
-    |> mem_insert 0x81000 8 0x82803
-    (* L2[0] -> L3 *)
-    |> mem_insert 0x82000 8 0x83803
-    (* L3[0] : map VA page 0x8000000000 -> PA page 0x0000 (executable) *)
-    |> mem_insert 0x83000 8 0x403
-    (* L3[1] : map VA page 0x8000001000 -> PA page 0x1000 (data) *)
-    |> mem_insert 0x83008 8 0x1443.
+  (* T1 Instructions *)
+  Definition instrs_t1 : list (bv addr_size * bv 32) :=
+    [(0x500, 0xf8206822); (* STR X2, [X1, X0] *)
+     (0x504, 0xf8236885)]. (* STR X5, [X4, X3] *)
+
+  (* T2 Instructions *)
+  Definition instrs_t2 : list (bv addr_size * bv 32) :=
+    [(0x600, 0xf8636885); (* LDR X5, [X4, X3] *)
+     (0x604, 0xf8606822)]. (* LDR X2, [X1, X0] *)
+
+  Definition data : list (bv addr_size * bv 64) :=
+    [(0x1100, 0x0); (0x1200, 0x0)].
+
+  (* Page Table *)
+  Definition pgt : list (bv addr_size * bv 64) :=
+    [(0x80008, 0x81803);
+     (0x81000, 0x82803);
+     (0x82000, 0x83803);
+     (0x83000, 0x403); (* PA page 0x0000 (executable, readable) *)
+     (0x83008, 0x60000000001443) (* PA page 0x1000 (data, readable, non-executable) *)].
 
   Definition n_threads := 2%nat.
 
@@ -401,7 +423,7 @@ Module MP.
   Definition mem_strict := false.
 
   Definition initState :=
-    {|archState.memory := init_mem;
+    {|archState.memory := init_vmem (instrs_t1 ++ instrs_t2) data pgt mem_strict;
       archState.regs := [# init_reg_t1; init_reg_t2];
       archState.address_space := PAS_NonSecure |}.
 
@@ -417,13 +439,9 @@ Module MP.
 End MP.
 
 Module MPDMBS.
-  (* A classic MP litmus test with address translation
+  (* A classic MPDMBS litmus test with address translation
      Thread 1: STR X2, [X1, X0]; DMB SY; STR X5, [X4, X3]
      Thread 2: LDR X5, [X4, X3]; DMB SY; LDR X2, [X1, X0]
-
-     VAs map to PAs:
-     - Instructions: 0x8000000500 -> 0x500, 0x8000000600 -> 0x600
-     - Data: 0x8000001100 -> 0x1100, 0x8000001200 -> 0x1200
 
      Expected outcome of (R5, R2) at Thread 2:
       (0x1, 0x2a), (0x0, 0x2a), (0x0, 0x0) *)
@@ -458,29 +476,28 @@ Module MPDMBS.
     |> reg_insert ID_AA64MMFR1_EL1 0x0
     |> reg_insert PSTATE (init_pstate 0%bv 0%bv).
 
-  Definition init_mem : memoryMap :=
-    ∅
-    (* Thread 1 @ PA 0x500 *)
-    |> mem_insert 0x500 4 0xf8206822  (* STR X2, [X1, X0] *)
-    |> mem_insert 0x504 4 0xd5033fbf  (* DMB SY *)
-    |> mem_insert 0x508 4 0xf8236885  (* STR X5, [X4, X3] *)
-    (* Thread 2 @ PA 0x600 *)
-    |> mem_insert 0x600 4 0xf8636885  (* LDR X5, [X4, X3] *)
-    |> mem_insert 0x604 4 0xd5033fbf  (* DMB SY *)
-    |> mem_insert 0x608 4 0xf8606822  (* LDR X2, [X1, X0] *)
-    (* Backing memory so the addresses exist *)
-    |> mem_insert 0x1100 8 0x0
-    |> mem_insert 0x1200 8 0x0
-    (* L0[1] -> L1  (for VA with L0 index = 1) *)
-    |> mem_insert 0x80008 8 0x81003
-    (* L1[0] -> L2 *)
-    |> mem_insert 0x81000 8 0x82003
-    (* L2[0] -> L3 *)
-    |> mem_insert 0x82000 8 0x83003
-    (* L3[0] : map VA page 0x8000000000 -> PA page 0x0000 (executable) *)
-    |> mem_insert 0x83000 8 0x403
-    (* L3[1] : map VA page 0x8000001000 -> PA page 0x1000 (data) *)
-    |> mem_insert 0x83008 8 0x60000000001443.
+  (* T1 Instructions *)
+  Definition instrs_t1 : list (bv addr_size * bv 32) :=
+    [(0x500, 0xf8206822);  (* STR X2, [X1, X0] *)
+     (0x504, 0xd5033fbf);  (* DMB SY *)
+     (0x508, 0xf8236885)]. (* STR X5, [X4, X3] *)
+
+  (* T2 Instructions *)
+  Definition instrs_t2 : list (bv addr_size * bv 32) :=
+    [(0x600, 0xf8636885);  (* LDR X5, [X4, X3] *)
+     (0x604, 0xd5033fbf);  (* DMB SY *)
+     (0x608, 0xf8606822)]. (* LDR X2, [X1, X0] *)
+
+  Definition data : list (bv addr_size * bv 64) :=
+    [(0x1100, 0x0); (0x1200, 0x0)].
+
+  (* Page Table *)
+  Definition pgt : list (bv addr_size * bv 64) :=
+    [(0x80008, 0x81803);
+     (0x81000, 0x82803);
+     (0x82000, 0x83803);
+     (0x83000, 0x403);
+     (0x83008, 0x60000000001443)].
 
   Definition n_threads := 2%nat.
 
@@ -495,10 +512,9 @@ Module MPDMBS.
   Definition mem_strict := false.
 
   Definition initState :=
-    {|archState.memory := init_mem;
+    {|archState.memory := init_vmem (instrs_t1 ++ instrs_t2) data pgt mem_strict;
       archState.regs := [# init_reg_t1; init_reg_t2];
       archState.address_space := PAS_NonSecure |}.
-
 
   Definition test_results :=
     VMPromising_cert_c_pf arm_sem fuel debug mem_strict n_threads termCond initState.
@@ -513,7 +529,7 @@ Module MPDMBS.
 End MPDMBS.
 
 (* Sequential page table modification in single thread *)
-Module BBM.
+Module BBMFailure.
   (* Single thread that:
      1. Loads from VA 0x8000001000 (gets 0x2a from PA 0x1000)
      2. Modifies L3[1] to remap VA 0x8000001000 -> PA 0x2000
@@ -534,34 +550,26 @@ Module BBM.
     |> reg_insert ID_AA64MMFR1_EL1 0x0
     |> reg_insert PSTATE (init_pstate 1%bv 1%bv).
 
-  Definition init_mem :=
-    ∅
-    (* Instructions
-      LDR X0, [X1, X0] - first load
-      STR X3, [X1, X2] - modify page table
-      LDR X4, [X1, X4] - second load *)
-    |> mem_insert 0x500 4 0xf8606820
-    |> mem_insert 0x504 4 0xf8226823
-    |> mem_insert 0x508 4 0xf8646824
-    (* Data at two different physical locations
-        Original PA - value 0x2a
-        New PA - value 0x42 *)
-    |> mem_insert 0x1000 8 0x2a
-    |> mem_insert 0x2000 8 0x42
-    (* Page tables
-        L0[1] -> L1
-        L1[0] -> L2
-        L2[0] -> L3
-        L3 entries:
-          - L3[0]  -> PA 0x0000 (code page for PC)
-          - L3[1]  -> PA 0x1000 (first data page), later updated to 0x2003 by the STR
-          - L3[16] -> PA 0x83000 (VA alias to edit L3 via VA 0x8000010000) *)
-    |> mem_insert 0x80008 8 0x81003
-    |> mem_insert 0x81000 8 0x82003
-    |> mem_insert 0x82000 8 0x83003
-    |> mem_insert 0x83000 8 0x40000000000783
-    |> mem_insert 0x83008 8 0x60000000001783
-    |> mem_insert 0x83080 8 0x60000000083703.
+  (* Instructions *)
+  Definition instrs : list (bv addr_size * bv 32) :=
+    [(0x500, 0xf8606820);  (* LDR X0, [X1, X0] - first load *)
+     (0x504, 0xf8226823);  (* STR X3, [X1, X2] - modify page table *)
+     (0x508, 0xf8646824)]. (* LDR X4, [X1, X4] - second load *)
+
+  (* Data at two different physical locations
+      Original PA - value 0x2a
+      New PA - value 0x42 *)
+  Definition data : list (bv addr_size * bv 64) :=
+    [(0x1000, 0x2a); (0x2000, 0x42)].
+
+  (* Page Table *)
+  Definition pgt : list (bv addr_size * bv 64) :=
+    [(0x80008, 0x81803);
+     (0x81000, 0x82003);
+     (0x82000, 0x83003);
+     (0x83000, 0x40000000000783);
+     (0x83008, 0x60000000001783);
+     (0x83080, 0x60000000083703)].
 
   Definition n_threads := 1%nat.
 
@@ -573,7 +581,7 @@ Module BBM.
   Definition mem_strict := false.
 
   Definition initState :=
-    {|archState.memory := init_mem;
+    {|archState.memory := init_vmem instrs data pgt mem_strict;
       archState.regs := [# init_reg];
       archState.address_space := PAS_NonSecure |}.
 
@@ -587,4 +595,102 @@ Module BBM.
     vm_compute (elements _).
     apply NoDup_Permutation; try solve_NoDup; set_solver.
   Qed.
-End BBM.
+End BBMFailure.
+
+(* Break-before-make success case *)
+Module BBMSuccess.
+  (* Thread 0:
+      - updates the last-level PTE for VA 0x8000001000
+      - executes a break-before-make sequence that only
+        invalidates the last-level mapping for that VA:
+        DSB ISHST; TLBI VAE1IS, X0; DSB ISH.
+    Thread 1:
+      - performs a data access via VA 0x8000001000. *)
+
+  Definition init_reg_t1 : registerMap :=
+    ∅
+    |> reg_insert _PC 0x8000000500
+    |> reg_insert R0 0x8000001000    (* VA to load from *)
+    |> reg_insert R1 0x0
+    |> reg_insert R2 0x8000010008    (* VA of L3[1] descriptor *)
+    |> reg_insert R3 0x0
+    |> reg_insert SCTLR_EL1 0x1
+    |> reg_insert TCR_EL1 0x0
+    |> reg_insert TTBR0_EL1 0x80000
+    |> reg_insert ID_AA64MMFR1_EL1 0x0
+    |> reg_insert PSTATE (init_pstate 1%bv 1%bv).
+
+  Definition init_reg_t2 : registerMap :=
+    ∅
+    |> reg_insert _PC 0x8000000600
+    |> reg_insert R0 0x8000001000    (* VA to load from *)
+    |> reg_insert R1 0x0
+    |> reg_insert SCTLR_EL1 0x1
+    |> reg_insert TCR_EL1 0x0
+    |> reg_insert TTBR0_EL1 0x80000
+    |> reg_insert ESR_EL1 0x0
+    |> reg_insert ID_AA64MMFR1_EL1 0x0
+    |> reg_insert PSTATE (init_pstate 1%bv 1%bv).
+
+  (* T1 Instructions *)
+  Definition instrs_t1 : list (bv addr_size * bv 32) :=
+    [(0x500, 0xf8226823);  (* STR X3, [X1, X2] - invalidate the PTE *)
+     (0x504, 0xd5033a9f);  (* DSB ISHST *)
+     (0x508, 0xd5088320);  (* TLBI by VA - TLB invalidate by 0x8000001000 *)
+     (0x50C, 0xd5033b9f);  (* DSB ISH *)
+     (0x510, 0xd5033fdf)]. (* ISB *)
+
+  (* T2 Instructions *)
+  Definition instrs_t2 : list (bv addr_size * bv 32) :=
+    [(0x600, 0xf8606820)]. (* LDR X0, [X1, X0] - read 0x8000001000 *)
+
+  (* Data - value 0x2a *)
+  Definition data : list (bv addr_size * bv 64) := [(0x1000, 0x2a)].
+
+  (* Page Table *)
+  Definition pgt : list (bv addr_size * bv 64) :=
+    [(0x80008, 0x81803);
+     (0x81000, 0x82003);
+     (0x82000, 0x83003);
+     (0x83000, 0x400000000000783);
+     (0x83008, 0x60000000001783);
+     (0x83080, 0x60000000083703)].
+
+  Definition n_threads := 2%nat.
+
+  Definition terminate_at_t1 rm : bool :=
+    reg_lookup _PC rm =? Some (0x800000050C : bv 64).
+
+  Definition terminate_at_t2 rm : bool :=
+    (* a valid translation *)
+    (reg_lookup _PC rm =? Some (0x8000000604 : bv 64))
+    (* or a fault *)
+    || ((reg_lookup FAR_EL1 rm =? Some (0x8000001000 : bv 64))
+        && (reg_lookup ELR_EL1 rm =? Some (0x8000000600 : bv 64))
+        && (reg_lookup ESR_EL1 rm =? Some (0x96000007 : bv 64))).
+
+  Definition terminate_at := [# terminate_at_t1; terminate_at_t2].
+
+  Definition termCond : terminationCondition n_threads :=
+    (λ tid rm, (terminate_at !!! tid) rm).
+
+  Definition fuel := 8%nat.
+  Definition debug := true.
+  Definition mem_strict := false.
+
+  Definition initState :=
+    {|archState.memory := init_vmem (instrs_t1 ++ instrs_t2) data pgt mem_strict;
+      archState.regs := [# init_reg_t1; init_reg_t2];
+      archState.address_space := PAS_NonSecure |}.
+
+  Definition test_results :=
+    VMPromising_cert_c_pf arm_sem fuel debug mem_strict n_threads termCond initState.
+
+  (* BBM check success *)
+  Goal elements (regs_extract [(1%fin, R0)] <$> test_results) ≡ₚ
+      [Ok [0x2a%Z]].
+  Proof.
+    vm_compute (elements _).
+    apply NoDup_Permutation; try solve_NoDup; set_solver.
+  Qed.
+End BBMSuccess.
